more adapting

Weidenbach_Book/code/full_SAT_Cached_Trail.sml
@@ -78,27 +78,19 @@ structure SAT_Solver : sig
   val integer_of_nat : nat -> IntInf.int
   val nat_of_integer : IntInf.int -> nat
   datatype int = Int_of_integer of IntInf.int
-  val integer_of_int : int -> IntInf.int
   type ('a, 'b) hashtable
-  val sAT_wl_code : (nat list) list -> (unit -> bool)
+  val integer_of_int : int -> IntInf.int
+  val uint32_of_nat : nat -> Word32.word
+  val sAT_wl_code : (Word32.word list) list -> (unit -> bool)
 end = struct
-
-datatype nat = Nat of IntInf.int;
-
-fun integer_of_nat (Nat x) = x;
-
-fun equal_nata m n = (((integer_of_nat m) : IntInf.int) = (integer_of_nat n));
-
-type 'a equal = {equal : 'a -> 'a -> bool};
-val equal = #equal : 'a equal -> 'a -> 'a -> bool;
-
-val equal_nat = {equal = equal_nata} : nat equal;
 
 datatype typerepa = Typerep of string * typerepa list;
 
 datatype num = One | Bit0 of num | Bit1 of num;
 
 datatype char = Zero_char | Char of num;
+
+datatype nat = Nat of IntInf.int;
 
 datatype 'a itself = Type;
 
@@ -134,6 +126,8 @@ val default = #default : 'a default -> 'a;
 
 val default_nat = {default = default_nata} : nat default;
 
+fun integer_of_nat (Nat x) = x;
+
 fun less_eq_nat m n = IntInf.<= (integer_of_nat m, integer_of_nat n);
 
 type 'a ord = {less_eq : 'a -> 'a -> bool, less : 'a -> 'a -> bool};
@@ -144,40 +138,13 @@ fun less_nat m n = IntInf.< (integer_of_nat m, integer_of_nat n);
 
 val ord_nat = {less_eq = less_eq_nat, less = less_nat} : nat ord;
 
-fun max A_ a b = (if less_eq A_ a b then b else a);
-
-val ord_integer =
-  {less_eq = (fn a => fn b => IntInf.<= (a, b)),
-    less = (fn a => fn b => IntInf.< (a, b))}
-  : IntInf.int ord;
-
-fun nat_of_integer k = Nat (max ord_integer (0 : IntInf.int) k);
-
-fun def_hashmap_size_nat x = (fn _ => nat_of_integer (16 : IntInf.int)) x;
-
-type 'a hashable =
-  {hashcode : 'a -> Word32.word, def_hashmap_size : 'a itself -> nat};
-val hashcode = #hashcode : 'a hashable -> 'a -> Word32.word;
-val def_hashmap_size = #def_hashmap_size : 'a hashable -> 'a itself -> nat;
-
-datatype int = Int_of_integer of IntInf.int;
-
-fun int_of_nat n = Int_of_integer (integer_of_nat n);
-
-fun integer_of_int (Int_of_integer k) = k;
-
-fun uint32_of_int i = Word32.fromLargeInt (IntInf.toLarge (integer_of_int i));
-
-fun hashcode_nat n = uint32_of_int (int_of_nat n);
-
-val hashable_nat =
-  {hashcode = hashcode_nat, def_hashmap_size = def_hashmap_size_nat} :
-  nat hashable;
-
 fun equal_boola p true = p
   | equal_boola p false = not p
   | equal_boola true p = p
   | equal_boola false p = not p;
+
+type 'a equal = {equal : 'a -> 'a -> bool};
+val equal = #equal : 'a equal -> 'a -> 'a -> bool;
 
 val equal_bool = {equal = equal_boola} : bool equal;
 
@@ -222,6 +189,50 @@ fun heap_option A_ =
     typerep_heap = typerep_option (typerep_heap A_)}
   : ('a option) heap;
 
+val equal_uint32 = {equal = (fn a => fn b => ((a : Word32.word) = b))} :
+  Word32.word equal;
+
+fun typerep_uint32a t = Typerep ("Uint32.uint32", []);
+
+val countable_uint32 = {} : Word32.word countable;
+
+val typerep_uint32 = {typerep = typerep_uint32a} : Word32.word typerep;
+
+val heap_uint32 =
+  {countable_heap = countable_uint32, typerep_heap = typerep_uint32} :
+  Word32.word heap;
+
+val default_uint32a : Word32.word = (Word32.fromInt 0);
+
+val default_uint32 = {default = default_uint32a} : Word32.word default;
+
+val ord_uint32 =
+  {less_eq = (fn a => fn b => Word32.<= (a, b)),
+    less = (fn a => fn b => Word32.< (a, b))}
+  : Word32.word ord;
+
+fun max A_ a b = (if less_eq A_ a b then b else a);
+
+val ord_integer =
+  {less_eq = (fn a => fn b => IntInf.<= (a, b)),
+    less = (fn a => fn b => IntInf.< (a, b))}
+  : IntInf.int ord;
+
+fun nat_of_integer k = Nat (max ord_integer (0 : IntInf.int) k);
+
+fun def_hashmap_size_uint32 x = (fn _ => nat_of_integer (16 : IntInf.int)) x;
+
+fun hashcode_uint32 n = n;
+
+type 'a hashable =
+  {hashcode : 'a -> Word32.word, def_hashmap_size : 'a itself -> nat};
+val hashcode = #hashcode : 'a hashable -> 'a -> Word32.word;
+val def_hashmap_size = #def_hashmap_size : 'a hashable -> 'a itself -> nat;
+
+val hashable_uint32 =
+  {hashcode = hashcode_uint32, def_hashmap_size = def_hashmap_size_uint32} :
+  Word32.word hashable;
+
 fun typerep_proda A_ B_ t =
   Typerep ("Product_Type.prod", [typerep A_ Type, typerep B_ Type]);
 
@@ -243,17 +254,26 @@ val typerep_unit = {typerep = typerep_unita} : unit typerep;
 val heap_unit = {countable_heap = countable_unit, typerep_heap = typerep_unit} :
   unit heap;
 
+datatype int = Int_of_integer of IntInf.int;
+
 datatype ('a, 'b) hashtable = HashTable of (('a * 'b) list) array * nat;
 
 fun eq A_ a b = equal A_ a b;
-
-fun nat k = Nat (max ord_integer (0 : IntInf.int) (integer_of_int k));
 
 fun plus_nat m n = Nat (IntInf.+ (integer_of_nat m, integer_of_nat n));
 
 val one_nat : nat = Nat (1 : IntInf.int);
 
 fun suc n = plus_nat n one_nat;
+
+fun minus_nat m n =
+  Nat (max ord_integer (0 : IntInf.int)
+        (IntInf.- (integer_of_nat m, integer_of_nat n)));
+
+fun equal_nat m n = (((integer_of_nat m) : IntInf.int) = (integer_of_nat n));
+
+fun nth (x :: xs) n =
+  (if equal_nat n zero_nata then x else nth xs (minus_nat n one_nat));
 
 fun len A_ a =
   (fn () => let
@@ -265,7 +285,7 @@ fun len A_ a =
 fun new A_ =
   (fn a => fn b => (fn () => Array.array (IntInf.toInt a, b))) o integer_of_nat;
 
-fun nth A_ a n = (fn () => Array.sub (a, IntInf.toInt (integer_of_nat n)));
+fun ntha A_ a n = (fn () => Array.sub (a, IntInf.toInt (integer_of_nat n)));
 
 fun upd A_ i x a =
   (fn () =>
@@ -287,12 +307,8 @@ fun hd (x21 :: x22) = x21;
 fun tl [] = []
   | tl (x21 :: x22) = x22;
 
-fun minus_nat m n =
-  Nat (max ord_integer (0 : IntInf.int)
-        (IntInf.- (integer_of_nat m, integer_of_nat n)));
-
 fun replicate n x =
-  (if equal_nata n zero_nata then []
+  (if equal_nat n zero_nata then []
     else x :: replicate (minus_nat n one_nat) x);
 
 fun is_none (SOME x) = false
@@ -381,7 +397,7 @@ fun ht_upd (A1_, A2_, A3_) B_ k v ht =
         val i = bounded_hashcode_nat A2_ m k;
       in
         (fn f_ => fn () => f_
-          ((nth (heap_list (heap_prod A3_ B_)) (the_array ht) i) ()) ())
+          ((ntha (heap_list (heap_prod A3_ B_)) (the_array ht) i) ()) ())
           (fn l =>
             let
               val la = ls_update A1_ k v l;
@@ -411,11 +427,11 @@ fun ht_insls (A1_, A2_, A3_) B_ [] ht = (fn () => ht)
               end);
 
 fun ht_copy (A1_, A2_, A3_) B_ n src dst =
-  (if equal_nata n zero_nata then (fn () => dst)
+  (if equal_nat n zero_nata then (fn () => dst)
     else (fn () =>
            let
              val l =
-               nth (heap_list (heap_prod A3_ B_)) (the_array src)
+               ntha (heap_list (heap_prod A3_ B_)) (the_array src)
                  (minus_nat n one_nat) ();
              val x = ht_insls (A1_, A2_, A3_) B_ l dst ();
            in
@@ -467,7 +483,7 @@ fun ht_lookup (A1_, A2_, A3_) B_ x ht =
         val i = bounded_hashcode_nat A2_ m x;
       in
         (fn f_ => fn () => f_
-          ((nth (heap_list (heap_prod A3_ B_)) (the_array ht) i) ()) ())
+          ((ntha (heap_list (heap_prod A3_ B_)) (the_array ht) i) ()) ())
           (fn l => (fn () => (ls_lookup A1_ x l)))
       end
         ()
@@ -477,12 +493,20 @@ fun op_list_hd x = hd x;
 
 fun op_list_tl x = tl x;
 
+fun integer_of_int (Int_of_integer k) = k;
+
+fun uint32_of_int i = Word32.fromLargeInt (IntInf.toLarge (integer_of_int i));
+
+fun int_of_nat n = Int_of_integer (integer_of_nat n);
+
+fun uint32_of_nat x = (uint32_of_int o int_of_nat) x;
+
 fun array_grow A_ a s x =
   (fn () =>
     let
       val l = len A_ a ();
     in
-      (if equal_nata l s then (fn () => a)
+      (if equal_nat l s then (fn () => a)
         else (fn f_ => fn () => f_ ((new A_ s x) ()) ())
                (fn aa =>
                  (fn f_ => fn () => f_ ((blit A_ a zero_nata aa zero_nata l) ())
@@ -498,13 +522,15 @@ fun hs_memb (A1_, A2_, A3_) x s =
               (case r of NONE => false | SOME _ => true)
             end);
 
+fun op_list_get x = nth x;
+
 fun array_copy A_ a =
   (fn () =>
     let
       val l = len A_ a ();
     in
-      (if equal_nata l zero_nata then (fn () => Array.fromList [])
-        else (fn f_ => fn () => f_ ((nth A_ a zero_nata) ()) ())
+      (if equal_nat l zero_nata then (fn () => Array.fromList [])
+        else (fn f_ => fn () => f_ ((ntha A_ a zero_nata) ()) ())
                (fn s =>
                  (fn f_ => fn () => f_ ((new A_ l s) ()) ())
                    (fn aa =>
@@ -514,12 +540,12 @@ fun array_copy A_ a =
         ()
     end);
 
-fun arl_get A_ = (fn (a, _) => nth A_ a);
+fun arl_get A_ = (fn (a, _) => ntha A_ a);
 
 fun nth_aa A_ xs i j =
   (fn () =>
     let
-      val x = nth (heap_prod (heap_array (typerep_heap A_)) heap_nat) xs i ();
+      val x = ntha (heap_prod (heap_array (typerep_heap A_)) heap_nat) xs i ();
       val xa = arl_get A_ x j ();
     in
       xa
@@ -530,9 +556,9 @@ fun array_shrink A_ a s =
     let
       val l = len A_ a ();
     in
-      (if equal_nata l s then (fn () => a)
-        else (if equal_nata l zero_nata then (fn () => Array.fromList [])
-               else (fn f_ => fn () => f_ ((nth A_ a zero_nata) ()) ())
+      (if equal_nat l s then (fn () => a)
+        else (if equal_nat l zero_nata then (fn () => Array.fromList [])
+               else (fn f_ => fn () => f_ ((ntha A_ a zero_nata) ()) ())
                       (fn x =>
                         (fn f_ => fn () => f_ ((new A_ s x) ()) ())
                           (fn aa =>
@@ -564,12 +590,12 @@ fun imp_for i u f s =
                      imp_for (plus_nat i one_nat) u f x ()
                    end));
 
-fun arl_last A_ = (fn (a, n) => nth A_ a (minus_nat n one_nat));
+fun arl_last A_ = (fn (a, n) => ntha A_ a (minus_nat n one_nat));
 
 fun last_aa A_ xs i =
   (fn () =>
     let
-      val x = nth (heap_prod (heap_array (typerep_heap A_)) heap_nat) xs i ();
+      val x = ntha (heap_prod (heap_array (typerep_heap A_)) heap_nat) xs i ();
     in
       arl_last A_ x ()
     end);
@@ -577,7 +603,7 @@ fun last_aa A_ xs i =
 fun nth_raa A_ xs i j =
   (fn () => let
               val x = arl_get (heap_array (typerep_heap A_)) xs i ();
-              val xa = nth A_ x j ();
+              val xa = ntha A_ x j ();
             in
               xa
             end);
@@ -635,7 +661,7 @@ fun arl_length A_ = (fn (_, a) => (fn () => a));
 fun length_aa A_ xs i =
   (fn () =>
     let
-      val x = nth (heap_prod (heap_array (typerep_heap A_)) heap_nat) xs i ();
+      val x = ntha (heap_prod (heap_array (typerep_heap A_)) heap_nat) xs i ();
     in
       arl_length A_ x ()
     end);
@@ -643,7 +669,7 @@ fun length_aa A_ xs i =
 fun update_aa A_ a i j y =
   (fn () =>
     let
-      val x = nth (heap_prod (heap_array (typerep_heap A_)) heap_nat) a i ();
+      val x = ntha (heap_prod (heap_array (typerep_heap A_)) heap_nat) a i ();
       val aa = arl_set A_ x j y ();
     in
       upd (heap_prod (heap_array (typerep_heap A_)) heap_nat) i aa a ()
@@ -713,7 +739,7 @@ fun arl_butlast A_ =
 
 fun is_None a = (case a of NONE => true | SOME _ => false);
 
-fun arl_is_empty A_ = (fn (_, n) => (fn () => (equal_nata n zero_nata)));
+fun arl_is_empty A_ = (fn (_, n) => (fn () => (equal_nat n zero_nata)));
 
 fun heap_WHILET b f s =
   (fn () =>
@@ -728,7 +754,7 @@ fun heap_WHILET b f s =
 fun append_el_aa (A1_, A2_) =
   (fn a => fn i => fn x => fn () =>
     let
-      val j = nth (heap_prod (heap_array (typerep_heap A2_)) heap_nat) a i ();
+      val j = ntha (heap_prod (heap_array (typerep_heap A2_)) heap_nat) a i ();
       val aa = arl_append (A1_, A2_) j x ();
     in
       upd (heap_prod (heap_array (typerep_heap A2_)) heap_nat) i aa a ()
@@ -737,17 +763,11 @@ fun append_el_aa (A1_, A2_) =
 fun set_butlast_aa A_ a i =
   (fn () =>
     let
-      val x = nth (heap_prod (heap_array (typerep_heap A_)) heap_nat) a i ();
+      val x = ntha (heap_prod (heap_array (typerep_heap A_)) heap_nat) a i ();
       val aa = arl_butlast A_ x ();
     in
       upd (heap_prod (heap_array (typerep_heap A_)) heap_nat) i aa a ()
     end);
-
-fun bitAND_int (Int_of_integer i) (Int_of_integer j) =
-  Int_of_integer (IntInf.andb (i, j));
-
-fun bitXOR_int (Int_of_integer i) (Int_of_integer j) =
-  Int_of_integer (IntInf.xorb (i, j));
 
 fun arl_of_array_raa A_ xs = (fn () => let
  val n = len A_ xs ();
@@ -794,14 +814,14 @@ fun arrayO_raa_empty_sz (A1_, A2_) B_ init_cap =
       (a, zero B_)
     end);
 
-fun bitAND_nat i j = nat (bitAND_int (int_of_nat i) (int_of_nat j));
-
-fun bitXOR_nat i j = nat (bitXOR_int (int_of_nat i) (int_of_nat j));
-
 fun equal_option A_ NONE (SOME x2) = false
   | equal_option A_ (SOME x2) NONE = false
   | equal_option A_ (SOME x2) (SOME y2) = eq A_ x2 y2
   | equal_option A_ NONE NONE = true;
+
+fun shiftr_uint32 x n =
+  (if less_nat n (nat_of_integer (32 : IntInf.int))
+    then Uint32.shiftr x (integer_of_nat n) else (Word32.fromInt 0));
 
 fun arrayO_ara_empty_sz_code (A1_, A2_) =
   (fn xi => fn () =>
@@ -820,37 +840,51 @@ fun decided l = (l, NONE);
 
 fun propagated l c = (l, SOME c);
 
+fun get_level_code x =
+  (fn ai => fn bi =>
+    let
+      val (_, (a1a, _)) = ai;
+    in
+      (fn () =>
+        let
+          val xa =
+            ntha (heap_prod (heap_option heap_bool) heap_nat) a1a
+              (nat_of_uint32 (shiftr_uint32 bi one_nat)) ();
+        in
+          snd xa
+        end)
+    end)
+    x;
+
 fun is_in_arl_code x =
   (fn ai => fn bi => fn () =>
     let
       val xa =
         heap_WHILET
           (fn s =>
-            (fn f_ => fn () => f_ ((arl_length heap_nat bi) ()) ())
+            (fn f_ => fn () => f_ ((arl_length heap_uint32 bi) ()) ())
               (fn xa =>
                 (if less_nat s xa
-                  then (fn f_ => fn () => f_ ((arl_get heap_nat bi s) ()) ())
-                         (fn xb => (fn () => (not (equal_nata xb ai))))
+                  then (fn f_ => fn () => f_ ((arl_get heap_uint32 bi s) ()) ())
+                         (fn xb => (fn () => (not ((xb : Word32.word) = ai))))
                   else (fn () => false))))
           (fn s => (fn () => (plus_nat s one_nat))) zero_nata ();
-      val x_a = arl_length heap_nat bi ();
+      val x_a = arl_length heap_uint32 bi ();
     in
       less_nat xa x_a
     end)
     x;
-
-fun uminus_lit_imp l = bitXOR_nat l one_nat;
 
 fun find_first_eq_code x =
   (fn ai => fn bi =>
     heap_WHILET
       (fn s => fn () =>
         let
-          val xa = arl_length heap_nat bi ();
+          val xa = arl_length heap_uint32 bi ();
         in
           (if less_nat s xa
-            then (fn f_ => fn () => f_ ((arl_get heap_nat bi s) ()) ())
-                   (fn xb => (fn () => (not (equal_nata xb ai))))
+            then (fn f_ => fn () => f_ ((arl_get heap_uint32 bi s) ()) ())
+                   (fn xb => (fn () => (not ((xb : Word32.word) = ai))))
             else (fn () => false))
             ()
         end)
@@ -861,20 +895,20 @@ fun remove1_wl_code x =
   (fn ai => fn bi => fn () =>
     let
       val xa = find_first_eq_code ai bi ();
-      val x_a = arl_length heap_nat bi ();
+      val x_a = arl_length heap_uint32 bi ();
     in
-      (if equal_nata xa x_a then (fn () => bi)
+      (if equal_nat xa x_a then (fn () => bi)
         else (fn f_ => fn () => f_
-               ((arl_swap heap_nat bi xa (minus_nat x_a one_nat)) ()) ())
-               (arl_butlast heap_nat))
+               ((arl_swap heap_uint32 bi xa (minus_nat x_a one_nat)) ()) ())
+               (arl_butlast heap_uint32))
         ()
     end)
     x;
 
 val extract_lits_clss_imp_empty_assn :
-  (unit -> ((nat, unit) hashtable * nat list))
+  (unit -> ((Word32.word, unit) hashtable * Word32.word list))
   = (fn () => let
-                val x = hs_new (hashable_nat, heap_nat) ();
+                val x = hs_new (hashable_uint32, heap_uint32) ();
               in
                 (x, [])
               end);
@@ -883,36 +917,38 @@ fun nat_lit_lits_init_assn_assn_prepend x =
   (fn ai => fn (a1, a2) => fn () =>
     let
       val xa =
-        hs_ins (equal_nat, hashable_nat, heap_nat)
-          ((nat_of_integer(IntInf.~>> (integer_of_nat(ai), Word.fromInt 1)))) a1
-          ();
+        hs_ins (equal_uint32, hashable_uint32, heap_uint32)
+          (shiftr_uint32 ai one_nat) a1 ();
     in
       (xa, op_list_prepend ai a2)
     end)
     x;
 
 fun nat_lit_lits_init_assn_assn_in x =
-  (fn ai => fn (a1, _) => hs_memb (equal_nat, hashable_nat, heap_nat) ai a1) x;
+  (fn ai => fn (a1, _) =>
+    hs_memb (equal_uint32, hashable_uint32, heap_uint32) ai a1)
+    x;
 
 fun extract_lits_cls_imp x =
   (fn ai =>
-    imp_nfoldli ai (fn _ => (fn () => true))
+    imp_for zero_nata (op_list_length ai)
       (fn xa => fn sigma => fn () =>
         let
-          val x_a =
+          val x_b =
             nat_lit_lits_init_assn_assn_in
-              ((nat_of_integer(IntInf.~>> (integer_of_nat(xa),
-                Word.fromInt 1))))
-              sigma ();
+              (shiftr_uint32 (op_list_get ai xa) one_nat) sigma ();
         in
-          (if x_a then (fn () => sigma)
-            else nat_lit_lits_init_assn_assn_prepend xa sigma)
+          (if x_b then (fn () => sigma)
+            else nat_lit_lits_init_assn_assn_prepend (op_list_get ai xa) sigma)
             ()
         end))
     x;
 
 fun extract_lits_clss_imp x =
-  (fn ai => imp_nfoldli ai (fn _ => (fn () => true)) extract_lits_cls_imp) x;
+  (fn ai =>
+    imp_for zero_nata (op_list_length ai)
+      (fn xa => extract_lits_cls_imp (op_list_get ai xa)))
+    x;
 
 fun extract_lits_clss_imp_list_assn x =
   (fn ai => fn bi => fn () => let
@@ -930,7 +966,7 @@ fun get_conflict_wl_is_None_code x =
                       end))
     x;
 
-fun hd_select_and_remove_from_pending_wl x =
+fun hd_select_and_remove_from_literals_to_update_wl x =
   ((fn a => (fn () => a)) o
     (fn (m, (n, (u, (d, (np, (up, (q, w))))))) =>
       ((m, (n, (u, (d, (np, (up, (tl q, w))))))), hd q)))
@@ -941,8 +977,11 @@ fun cons_trail_Propagated_tr_code x =
     let
       val xa =
         upd (heap_prod (heap_option heap_bool) heap_nat)
-          ((nat_of_integer(IntInf.~>> (integer_of_nat(ai), Word.fromInt 1))))
-          (SOME (equal_nata (bitAND_nat ai one_nat) zero_nata), a2a) a1a ();
+          (nat_of_uint32 (shiftr_uint32 ai one_nat))
+          (SOME (((Word32.andb (ai,
+                    (Word32.fromInt 1))) : Word32.word) = (Word32.fromInt 0)),
+            a2a)
+          a1a ();
     in
       (op_list_prepend (propagated ai bia) a1, (xa, a2a))
     end)
@@ -964,31 +1003,31 @@ fun valued_trail_code x =
       (fn () =>
         let
           val xa =
-            nth (heap_prod (heap_option heap_bool) heap_nat) a1a
-              ((nat_of_integer(IntInf.~>> (integer_of_nat(bi),
-                Word.fromInt 1))))
-              ();
+            ntha (heap_prod (heap_option heap_bool) heap_nat) a1a
+              (nat_of_uint32 (shiftr_uint32 bi one_nat)) ();
         in
           (case fst xa of NONE => NONE
             | SOME x_a =>
-              (if equal_nata (bitAND_nat bi one_nat) zero_nata then SOME x_a
-                else SOME (not x_a)))
+              (if (((Word32.andb (bi,
+                      (Word32.fromInt 1))) : Word32.word) = (Word32.fromInt 0))
+                then SOME x_a else SOME (not x_a)))
         end)
     end)
     x;
 
 fun find_unwatched_code x =
   (fn ai => fn bia => fn bi =>
-    heap_WHILET (fn (a1, a2) => fn () => let
-   val xa = nth_rl heap_nat bia bi ();
-   val xb = len heap_nat xa ();
- in
-   is_none a1 andalso less_nat a2 xb
- end)
+    heap_WHILET
+      (fn (a1, a2) => fn () => let
+                                 val xa = nth_rl heap_uint32 bia bi ();
+                                 val xb = len heap_uint32 xa ();
+                               in
+                                 is_none a1 andalso less_nat a2 xb
+                               end)
       (fn (_, a2) => fn () =>
         let
-          val xa = nth_rl heap_nat bia bi ();
-          val xb = nth heap_nat xa a2 ();
+          val xa = nth_rl heap_uint32 bia bi ();
+          val xb = ntha heap_uint32 xa a2 ();
           val x_a = valued_trail_code ai xb ();
         in
           (case x_a of NONE => (SOME false, a2) | SOME true => (SOME true, a2)
@@ -1001,14 +1040,14 @@ fun unit_propagation_inner_loop_body_wl_D_code x =
   (fn ai => fn bia => fn (a1, (a1a, (a1b, (a1c, (a1d, (a1e, (a1f, a2f))))))) =>
     fn () =>
     let
-      val x_a = nth_aa heap_nat a2f ai bia ();
-      val xa = nth_raa heap_nat a1a x_a zero_nata ();
+      val x_a = nth_aa heap_nat a2f (nat_of_uint32 ai) bia ();
+      val xa = nth_raa heap_uint32 a1a x_a zero_nata ();
     in
       let
-        val x_c = (if equal_nata xa ai then zero_nata else one_nat);
+        val x_c = (if ((xa : Word32.word) = ai) then zero_nata else one_nat);
       in
         (fn f_ => fn () => f_
-          ((nth_raa heap_nat a1a x_a (minus_nat one_nat x_c)) ()) ())
+          ((nth_raa heap_uint32 a1a x_a (minus_nat one_nat x_c)) ()) ())
           (fn x_f =>
             (fn f_ => fn () => f_ ((valued_trail_code a1 x_f) ()) ())
               (fn x_h =>
@@ -1022,9 +1061,9 @@ fun unit_propagation_inner_loop_body_wl_D_code x =
                            (if is_none (fst x_j)
                              then (if equal_option equal_bool x_h (SOME false)
                                     then (fn f_ => fn () => f_
-   ((nth_rl heap_nat a1a x_a) ()) ())
+   ((nth_rl heap_uint32 a1a x_a) ()) ())
    (fn xb =>
-     (fn f_ => fn () => f_ ((arl_of_array_raa heap_nat xb) ()) ())
+     (fn f_ => fn () => f_ ((arl_of_array_raa heap_uint32 xb) ()) ())
        (fn xc =>
          (fn () =>
            (plus_nat bia one_nat,
@@ -1035,18 +1074,20 @@ fun unit_propagation_inner_loop_body_wl_D_code x =
      (fn () =>
        (plus_nat bia one_nat,
          (xb, (a1a, (a1b, (a1c, (a1d, (a1e,
-(uminus_lit_imp x_f :: a1f, a2f)))))))))))
+(Word32.xorb (x_f, (Word32.fromInt 1)) :: a1f, a2f)))))))))))
                              else (fn f_ => fn () => f_
-                                    ((nth_raa heap_nat a1a x_a (snd x_j)) ())
+                                    ((nth_raa heap_uint32 a1a x_a (snd x_j)) ())
                                     ())
                                     (fn x_l =>
                                       (fn f_ => fn () => f_
-((swap_aa (default_nat, heap_nat) a1a x_a x_c (snd x_j)) ()) ())
+((swap_aa (default_uint32, heap_uint32) a1a x_a x_c (snd x_j)) ()) ())
 (fn x_n =>
-  (fn f_ => fn () => f_ ((delete_index_and_swap_aa heap_nat a2f ai bia) ()) ())
+  (fn f_ => fn () => f_
+    ((delete_index_and_swap_aa heap_nat a2f (nat_of_uint32 ai) bia) ()) ())
     (fn x_p =>
-      (fn f_ => fn () => f_ ((append_el_aa (default_nat, heap_nat) x_p x_l x_a)
-        ()) ())
+      (fn f_ => fn () => f_
+        ((append_el_aa (default_nat, heap_nat) x_p (nat_of_uint32 x_l) x_a) ())
+        ())
         (fn x_r =>
           (fn () =>
             (bia, (a1, (x_n, (a1b, (a1c, (a1d, (a1e, (a1f, x_r))))))))))))))))))
@@ -1060,7 +1101,7 @@ fun unit_propagation_inner_loop_wl_loop_D_code x =
     heap_WHILET
       (fn (a1, (_, (_, (_, (a1d, (_, (_, (_, a2g)))))))) => fn () =>
         let
-          val xa = length_aa heap_nat a2g ai ();
+          val xa = length_aa heap_nat a2g (nat_of_uint32 ai) ();
         in
           less_nat a1 xa andalso is_None a1d
         end)
@@ -1077,27 +1118,28 @@ fun unit_propagation_inner_loop_wl_D_code x =
     end)
     x;
 
-fun pending_wll_empty x =
+fun literals_to_update_wll_empty x =
   ((fn a => (fn () => a)) o
     (fn (_, (_, (_, (_, (_, (_, (q, _))))))) => is_Nil q))
     x;
 
 fun unit_propagation_outer_loop_wl_D_code x =
   heap_WHILET (fn s => fn () => let
-                                  val xa = pending_wll_empty s ();
+                                  val xa = literals_to_update_wll_empty s ();
                                 in
                                   not xa
                                 end)
-    (fn s => fn () => let
-                        val a = hd_select_and_remove_from_pending_wl s ();
-                      in
-                        let
-                          val (a1, a2) = a;
-                        in
-                          unit_propagation_inner_loop_wl_D_code a2 a1
-                        end
-                          ()
-                      end)
+    (fn s => fn () =>
+      let
+        val a = hd_select_and_remove_from_literals_to_update_wl s ();
+      in
+        let
+          val (a1, a2) = a;
+        in
+          unit_propagation_inner_loop_wl_D_code a2 a1
+        end
+          ()
+      end)
     x;
 
 fun is_decided_wl_code x = (fn xi => (fn () => (is_None (snd xi)))) x;
@@ -1114,60 +1156,44 @@ fun is_decided_hd_trail_wll_code x =
 fun get_conflict_wll_is_Nil_code x =
   (fn (_, (_, (_, (a1c, (_, (_, (_, _))))))) =>
     (if is_None a1c then (fn () => false)
-      else (arl_is_empty heap_nat o the) a1c))
+      else (arl_is_empty heap_uint32 o the) a1c))
     x;
 
 fun union_mset_list_fold_code x =
   (fn ai => fn bi => fn () =>
     let
-      val xa = arl_copy heap_nat ai ();
-      val xaa = arl_length heap_nat bi ();
+      val xa = arl_copy heap_uint32 ai ();
+      val xaa = arl_length heap_uint32 bi ();
     in
       imp_for zero_nata xaa
         (fn xb => fn sigma =>
-          (fn f_ => fn () => f_ ((arl_get heap_nat bi xb) ()) ())
+          (fn f_ => fn () => f_ ((arl_get heap_uint32 bi xb) ()) ())
             (fn xab =>
               (fn f_ => fn () => f_ ((is_in_arl_code xab xa) ()) ())
                 (fn x_c =>
                   (if x_c then (fn () => sigma)
-                    else (fn f_ => fn () => f_ ((arl_get heap_nat bi xb) ()) ())
-                           (arl_append (default_nat, heap_nat) sigma)))))
+                    else (fn f_ => fn () => f_ ((arl_get heap_uint32 bi xb) ())
+                           ())
+                           (arl_append (default_uint32, heap_uint32) sigma)))))
         ai ()
-    end)
-    x;
-
-fun get_level_code_get_level_code x =
-  (fn ai => fn bi =>
-    let
-      val (_, (a1a, _)) = ai;
-    in
-      (fn () =>
-        let
-          val xa =
-            nth (heap_prod (heap_option heap_bool) heap_nat) a1a
-              ((nat_of_integer(IntInf.~>> (integer_of_nat(bi),
-                Word.fromInt 1))))
-              ();
-        in
-          snd xa
-        end)
     end)
     x;
 
 fun maximum_level_remove_code x =
   (fn ai => fn bia => fn bi => fn () =>
     let
-      val xa = arl_length heap_nat bia ();
+      val xa = arl_length heap_uint32 bia ();
       val xb =
         imp_for zero_nata xa
           (fn xb => fn (a1, a2) =>
-            (fn f_ => fn () => f_ ((arl_get heap_nat bia xb) ()) ())
+            (fn f_ => fn () => f_ ((arl_get heap_uint32 bia xb) ()) ())
               (fn xc =>
-                (if equal_nata xc bi andalso not a1 then (fn () => (true, a2))
-                  else (fn f_ => fn () => f_ ((arl_get heap_nat bia xb) ()) ())
+                (if ((xc : Word32.word) = bi) andalso not a1
+                  then (fn () => (true, a2))
+                  else (fn f_ => fn () => f_ ((arl_get heap_uint32 bia xb) ())
+                         ())
                          (fn xd =>
-                           (fn f_ => fn () => f_
-                             ((get_level_code_get_level_code ai xd) ()) ())
+                           (fn f_ => fn () => f_ ((get_level_code ai xd) ()) ())
                              (fn xe => (fn () => (a1, max ord_nat xe a2)))))))
           (false, zero_nata) ();
     in
@@ -1180,8 +1206,7 @@ fun tl_trail_tr_code x =
     let
       val xa =
         upd (heap_prod (heap_option heap_bool) heap_nat)
-          ((nat_of_integer(IntInf.~>> (integer_of_nat(fst (op_list_hd a1)),
-            Word.fromInt 1))))
+          (nat_of_uint32 (shiftr_uint32 (fst (op_list_hd a1)) one_nat))
           (NONE, zero_nata) a1a ();
       val xaa = is_decided_wl_code (op_list_hd a1) ();
     in
@@ -1212,7 +1237,9 @@ fun skip_and_resolve_loop_wl_D_code x =
                     val (a1h, a2h) = (fst xb, the (snd xb));
                   in
                     (fn f_ => fn () => f_
-                      ((is_in_arl_code (uminus_lit_imp a1h) x_b) ()) ())
+                      ((is_in_arl_code (Word32.xorb (a1h, (Word32.fromInt 1)))
+                         x_b)
+                      ()) ())
                       (fn xc =>
                         (if not xc
                           then (fn f_ => fn () => f_ ((tl_trail_tr_code a1a) ())
@@ -1224,30 +1251,30 @@ fun skip_and_resolve_loop_wl_D_code x =
  (a1b, (a1c, (SOME x_b, (a1e, (a1f, (a1g, a2g))))))))))
                           else (fn f_ => fn () => f_
                                  ((maximum_level_remove_code a1a x_b
-                                    (uminus_lit_imp a1h))
+                                    (Word32.xorb (a1h, (Word32.fromInt 1))))
                                  ()) ())
                                  (fn xd =>
-                                   (if equal_nata xd let
-               val (_, (_, k)) = a1a;
-             in
-               k
-             end
+                                   (if equal_nat xd let
+              val (_, (_, k)) = a1a;
+            in
+              k
+            end
                                      then (fn f_ => fn () => f_
-    ((remove1_wl_code (uminus_lit_imp a1h) x_b) ()) ())
+    ((remove1_wl_code (Word32.xorb (a1h, (Word32.fromInt 1))) x_b) ()) ())
     (fn x_h =>
       (fn f_ => fn () => f_
-        ((if equal_nata a2h zero_nata
-           then arl_empty (default_nat, heap_nat) zero_nat
-           else (fn f_ => fn () => f_ ((nth_rl heap_nat a1b a2h) ()) ())
+        ((if equal_nat a2h zero_nata
+           then arl_empty (default_uint32, heap_uint32) zero_nat
+           else (fn f_ => fn () => f_ ((nth_rl heap_uint32 a1b a2h) ()) ())
                   (fn xe =>
-                    (fn f_ => fn () => f_ ((arl_of_array_raa heap_nat xe) ())
+                    (fn f_ => fn () => f_ ((arl_of_array_raa heap_uint32 xe) ())
                       ())
                       (remove1_wl_code a1h)))
         ()) ())
         (fn x_j =>
           (fn f_ => fn () => f_ ((union_mset_list_fold_code x_h x_j) ()) ())
             (fn x_l =>
-              (fn f_ => fn () => f_ ((arl_is_empty heap_nat x_l) ()) ())
+              (fn f_ => fn () => f_ ((arl_is_empty heap_uint32 x_l) ()) ())
                 (fn x_n =>
                   (fn f_ => fn () => f_ ((tl_trail_tr_code a1a) ()) ())
                     (fn xe =>
@@ -1293,8 +1320,9 @@ fun cons_trail_Decided_tr_code x =
     let
       val xa =
         upd (heap_prod (heap_option heap_bool) heap_nat)
-          ((nat_of_integer(IntInf.~>> (integer_of_nat(ai), Word.fromInt 1))))
-          (SOME (equal_nata (bitAND_nat ai one_nat) zero_nata),
+          (nat_of_uint32 (shiftr_uint32 ai one_nat))
+          (SOME (((Word32.andb (ai,
+                    (Word32.fromInt 1))) : Word32.word) = (Word32.fromInt 0)),
             plus_nat a2a one_nat)
           a1a ();
     in
@@ -1318,7 +1346,7 @@ fun decide_wl_or_skip_D_code n_0 =
                    (fn () =>
                      (false,
                        (xa, (a1a, (a1b, (a1c,
-  (a1d, (a1e, ([uminus_lit_imp x_c], a2f))))))))))
+  (a1d, (a1e, ([Word32.xorb (x_c, (Word32.fromInt 1))], a2f))))))))))
              end
         else (fn () => (true, xi)))
         ()
@@ -1328,23 +1356,25 @@ fun find_lit_of_max_level_wl_imp_code x =
   (fn ai => fn _ => fn _ => fn bie => fn _ => fn _ => fn _ => fn _ => fn bi =>
     fn () =>
     let
-      val xa = maximum_level_remove_code ai bie (uminus_lit_imp bi) ();
+      val xa =
+        maximum_level_remove_code ai bie (Word32.xorb (bi, (Word32.fromInt 1)))
+          ();
       val xb =
         heap_WHILET
           (fn s =>
-            (fn f_ => fn () => f_ ((arl_get heap_nat bie s) ()) ())
+            (fn f_ => fn () => f_ ((arl_get heap_uint32 bie s) ()) ())
               (fn xaa =>
-                (fn f_ => fn () => f_ ((arl_get heap_nat bie s) ()) ())
+                (fn f_ => fn () => f_ ((arl_get heap_uint32 bie s) ()) ())
                   (fn xb =>
-                    (fn f_ => fn () => f_ ((get_level_code_get_level_code ai xb)
-                      ()) ())
+                    (fn f_ => fn () => f_ ((get_level_code ai xb) ()) ())
                       (fn xba =>
                         (fn () =>
-                          (if not (equal_nata xaa (uminus_lit_imp bi))
-                            then not (equal_nata xba xa) else true))))))
+                          (if not ((xaa : Word32.word) = (Word32.xorb (bi,
+                   (Word32.fromInt 1))))
+                            then not (equal_nat xba xa) else true))))))
           (fn s => (fn () => (plus_nat s one_nat))) zero_nata ();
     in
-      arl_get heap_nat bie xb ()
+      arl_get heap_uint32 bie xb ()
     end)
     x;
 
@@ -1353,17 +1383,19 @@ fun remove1_and_add_first_code x =
     let
       val xa = find_first_eq_code ai bi ();
       val x_b = find_first_eq_code bia bi ();
-      val x_d = arl_swap heap_nat bi zero_nata xa ();
+      val x_d = arl_swap heap_uint32 bi zero_nata xa ();
     in
-      arl_swap heap_nat x_d one_nat
-        (if equal_nata x_b zero_nata then xa else x_b) ()
+      arl_swap heap_uint32 x_d one_nat
+        (if equal_nat x_b zero_nata then xa else x_b) ()
     end)
     x;
 
 fun find_decomp_wl_imp_code x =
   (fn ai => fn bia => fn bi => fn () =>
     let
-      val xa = maximum_level_remove_code ai bia (uminus_lit_imp bi) ();
+      val xa =
+        maximum_level_remove_code ai bia (Word32.xorb (bi, (Word32.fromInt 1)))
+          ();
       val a =
         heap_WHILET (fn (a1, _) => (fn () => (less_nat xa a1)))
           (fn (a1, a2) =>
@@ -1399,7 +1431,7 @@ fun find_decomp_wl_imp_codea x =
     find_decomp_wl_imp_code ai bie)
     x;
 
-fun single_of_mset_imp_code x = (fn xi => arl_get heap_nat xi zero_nata) x;
+fun single_of_mset_imp_code x = (fn xi => arl_get heap_uint32 xi zero_nata) x;
 
 fun backtrack_wl_D_code x =
   (fn (a1, (a1a, (a1b, (a1c, (a1d, (a1e, (a1f, a2f))))))) => fn () =>
@@ -1413,7 +1445,7 @@ fun backtrack_wl_D_code x =
         (fn f_ => fn () => f_
           ((find_decomp_wl_imp_codea a1 a1a a1b x_c a1d a1e a1f a2f x_a) ()) ())
           (fn x_e =>
-            (fn f_ => fn () => f_ ((arl_length heap_nat x_c) ()) ())
+            (fn f_ => fn () => f_ ((arl_length heap_uint32 x_c) ()) ())
               (fn xb =>
                 (if less_nat one_nat xb
                   then (fn f_ => fn () => f_
@@ -1422,34 +1454,38 @@ fun backtrack_wl_D_code x =
                          ()) ())
                          (fn x_g =>
                            (fn f_ => fn () => f_
-                             ((remove1_and_add_first_code (uminus_lit_imp x_a)
-                                x_g x_c)
+                             ((remove1_and_add_first_code
+                                (Word32.xorb (x_a, (Word32.fromInt 1))) x_g x_c)
                              ()) ())
                              (fn x_j =>
-                               (fn f_ => fn () => f_ ((length_ra heap_nat a1a)
-                                 ()) ())
+                               (fn f_ => fn () => f_
+                                 ((length_ra heap_uint32 a1a) ()) ())
                                  (fn xc =>
                                    (fn f_ => fn () => f_
                                      ((append_el_aa (default_nat, heap_nat) a2f
-x_g xc)
+(nat_of_uint32 x_g) xc)
                                      ()) ())
                                      (fn x_k =>
                                        (fn f_ => fn () => f_
- ((length_ra heap_nat a1a) ()) ())
+ ((length_ra heap_uint32 a1a) ()) ())
  (fn xd =>
    (fn f_ => fn () => f_
-     ((append_el_aa (default_nat, heap_nat) x_k (uminus_lit_imp x_a) xd) ()) ())
+     ((append_el_aa (default_nat, heap_nat) x_k
+        (nat_of_uint32 (Word32.xorb (x_a, (Word32.fromInt 1)))) xd)
+     ()) ())
      (fn x_m =>
-       (fn f_ => fn () => f_ ((length_ra heap_nat a1a) ()) ())
+       (fn f_ => fn () => f_ ((length_ra heap_uint32 a1a) ()) ())
          (fn xe =>
            (fn f_ => fn () => f_
-             ((cons_trail_Propagated_tr_code (uminus_lit_imp x_a) xe x_e) ())
-             ())
+             ((cons_trail_Propagated_tr_code
+                (Word32.xorb (x_a, (Word32.fromInt 1))) xe x_e)
+             ()) ())
              (fn x_o =>
-               (fn f_ => fn () => f_ ((array_of_arl_raa heap_nat x_j) ()) ())
+               (fn f_ => fn () => f_ ((array_of_arl_raa heap_uint32 x_j) ()) ())
                  (fn xf =>
                    (fn f_ => fn () => f_
-                     ((arrayO_raa_append (default_nat, heap_nat) a1a xf) ()) ())
+                     ((arrayO_raa_append (default_uint32, heap_uint32) a1a xf)
+                     ()) ())
                      (fn xg =>
                        (fn () =>
                          (x_o, (xg, (a1b, (NONE,
@@ -1459,7 +1495,8 @@ x_g xc)
                          (fn x_g =>
                            (fn f_ => fn () => f_
                              ((cons_trail_Propagated_tr_code
-                                (uminus_lit_imp x_a) zero_nata x_e)
+                                (Word32.xorb (x_a, (Word32.fromInt 1)))
+                                zero_nata x_e)
                              ()) ())
                              (fn x_h =>
                                (fn () =>
@@ -1508,26 +1545,28 @@ fun cdcl_twl_stgy_prog_wl_D_code n_0 =
         ()
     end);
 
-fun init_state_wl_D n l_Ns =
+fun init_state_wl_D n_0 l_Ns =
   let
-    val na = suc (suc (fold (max ord_nat) n zero_nata));
+    val n =
+      suc (suc (nat_of_uint32 (fold (max ord_uint32) n_0 (Word32.fromInt 0))));
   in
     (fn () =>
       let
-        val naa = arrayO_raa_empty_sz (default_nat, heap_nat) zero_nat l_Ns ();
-        val e = new heap_nat zero_nata zero_nata ();
-        val nab = arrayO_raa_append (default_nat, heap_nat) naa e ();
-        val ws = arrayO_ara_empty_sz_code (default_nat, heap_nat) na ();
+        val na =
+          arrayO_raa_empty_sz (default_uint32, heap_uint32) zero_nat l_Ns ();
+        val e = new heap_uint32 zero_nata (Word32.fromInt 0) ();
+        val naa = arrayO_raa_append (default_uint32, heap_uint32) na e ();
+        val ws = arrayO_ara_empty_sz_code (default_nat, heap_nat) n ();
         val m =
           new (heap_prod (heap_option heap_bool) heap_nat)
-            ((nat_of_integer(IntInf.~>> (integer_of_nat(na), Word.fromInt 1))))
+            ((nat_of_integer(IntInf.~>> (integer_of_nat(n), Word.fromInt 1))))
             (NONE, zero_nata) ();
       in
-        (([], (m, zero_nata)), (nab, (zero_nata, (NONE, ([], ([], ([], ws)))))))
+        (([], (m, zero_nata)), (naa, (zero_nata, (NONE, ([], ([], ([], ws)))))))
       end)
   end;
 
-fun init_state_wl_D_code n = init_state_wl_D n;
+fun init_state_wl_D_code n_0 = init_state_wl_D n_0;
 
 fun arl_of_list_raa A_ xs =
   (fn () => let
@@ -1540,7 +1579,7 @@ fun init_dt_step_wl_code x =
   (fn _ => fn bia => fn a =>
     (case a
       of (a1, (a1a, (a1b, (NONE, (a1d, (a1e, (a1f, a2f))))))) =>
-        (if equal_nata (op_list_length bia) one_nat
+        (if equal_nat (op_list_length bia) one_nat
           then let
                  val x_b = op_list_hd bia;
                in
@@ -1555,13 +1594,15 @@ fun init_dt_step_wl_code x =
                               (fn x_g =>
                                 (fn () =>
                                   (x_g, (a1a,
-  (a1b, (NONE, ([x_b] :: a1d, (a1e, (uminus_lit_imp x_b :: a1f, a2f)))))))))
+  (a1b, (NONE,
+          ([x_b] :: a1d,
+            (a1e, (Word32.xorb (x_b, (Word32.fromInt 1)) :: a1f, a2f)))))))))
                        else (if equal_option equal_bool x_d (SOME true)
                               then (fn () =>
                                      (a1, (a1a,
     (a1b, (NONE, ([x_b] :: a1d, (a1e, (a1f, a2f))))))))
                               else (fn f_ => fn () => f_
-                                     ((arl_of_list_raa heap_nat bia) ()) ())
+                                     ((arl_of_list_raa heap_uint32 bia) ()) ())
                                      (fn xa =>
                                        (fn () =>
  (a1, (a1a, (a1b, (SOME xa, ([x_b] :: a1d, (a1e, ([], a2f)))))))))))
@@ -1570,35 +1611,37 @@ fun init_dt_step_wl_code x =
                end
           else (fn () =>
                  let
-                   val x_b = length_ra heap_nat a1a ();
+                   val x_b = length_ra heap_uint32 a1a ();
                    val x_d =
-                     append_el_aa (default_nat, heap_nat) a2f (op_list_hd bia)
-                       x_b ();
+                     append_el_aa (default_nat, heap_nat) a2f
+                       (nat_of_uint32 (op_list_hd bia)) x_b ();
                    val x_f =
                      append_el_aa (default_nat, heap_nat) x_d
-                       (op_list_hd (op_list_tl bia)) x_b ();
+                       (nat_of_uint32 (op_list_hd (op_list_tl bia))) x_b ();
                    val xa = (fn () => Array.fromList bia) ();
-                   val xb = arrayO_raa_append (default_nat, heap_nat) a1a xa ();
+                   val xb =
+                     arrayO_raa_append (default_uint32, heap_uint32) a1a xa ();
                  in
                    (a1, (xb, (x_b, (NONE, (a1d, (a1e, (a1f, x_f)))))))
                  end))
       | (a1, (a1a, (a1b, (SOME x_a, (a1d, (a1e, (_, a2f))))))) =>
-        (if equal_nata (op_list_length bia) one_nat
+        (if equal_nat (op_list_length bia) one_nat
           then (fn () =>
                  (a1, (a1a, (a1b, (SOME x_a,
                                     ([op_list_hd bia] :: a1d,
                                       (a1e, ([], a2f))))))))
           else (fn () =>
                  let
-                   val x_c = length_ra heap_nat a1a ();
+                   val x_c = length_ra heap_uint32 a1a ();
                    val x_e =
-                     append_el_aa (default_nat, heap_nat) a2f (op_list_hd bia)
-                       x_c ();
+                     append_el_aa (default_nat, heap_nat) a2f
+                       (nat_of_uint32 (op_list_hd bia)) x_c ();
                    val x_g =
                      append_el_aa (default_nat, heap_nat) x_e
-                       (op_list_hd (op_list_tl bia)) x_c ();
+                       (nat_of_uint32 (op_list_hd (op_list_tl bia))) x_c ();
                    val xa = (fn () => Array.fromList bia) ();
-                   val xb = arrayO_raa_append (default_nat, heap_nat) a1a xa ();
+                   val xb =
+                     arrayO_raa_append (default_uint32, heap_uint32) a1a xa ();
                  in
                    (a1, (xb, (x_c, (SOME x_a, (a1d, (a1e, ([], x_g)))))))
                  end))))
