Weidenbach_Book/CDCL_Two_Watched_Literals_List_Watched_Code_Common.thy
@@ -117,14 +117,6 @@ subsection \<open>State Conversion\<close>
 subsubsection \<open>Functions and Types:\<close>
 
 type_synonym clauses_wl = \<open>uint32 arrayO_raa\<close>
-
-text \<open>TODO Move\<close>
-abbreviation uint32_rel :: \<open>(uint32 \<times> uint32) set\<close> where
-  \<open>uint32_rel \<equiv> Id\<close>
-
-abbreviation uint32_assn :: \<open>uint32 \<Rightarrow> uint32 \<Rightarrow> assn\<close> where
-  \<open>uint32_assn \<equiv> id_assn\<close>
-
 abbreviation ann_lit_wl_assn :: \<open>ann_lit_wl \<Rightarrow> ann_lit_wl \<Rightarrow> assn\<close> where
   \<open>ann_lit_wl_assn \<equiv> prod_assn uint32_assn (option_assn nat_assn)\<close>
 
@@ -1306,9 +1298,6 @@ lemma find_decomp_wl_imp_find_decomp_wl':
     by (cases S, cases S') (auto intro!: find_decomp_wl_code_find_decomp_wl)
   done
 
-context twl_array_code
-begin
-
 definition get_conflict_wl_is_None :: \<open>nat twl_st_wl \<Rightarrow> bool\<close> where
   \<open>get_conflict_wl_is_None = (\<lambda>(M, N, U, D, NP, UP, Q, W). is_None D)\<close>
 
@@ -1319,6 +1308,9 @@ lemma watched_by_nth_watched_app':
   \<open>watched_by S K = ((snd o snd o snd o snd o snd o snd o snd) S) K\<close>
   by (cases S) (auto simp: watched_app_def)
 
+
+context twl_array_code
+begin
 
 sepref_definition (in -) find_decomp_wl_imp_code
   is \<open>uncurry2 (find_decomp_wl_imp)\<close>
@@ -1520,7 +1512,7 @@ proof -
     using H unfolding pre init .
 qed
 
-definition append_update :: "('a \<Rightarrow> 'b list) \<Rightarrow> 'a \<Rightarrow> 'b \<Rightarrow> 'a \<Rightarrow> 'b list"  where
+definition (in twl_array_code_ops) append_update :: "('a \<Rightarrow> 'b list) \<Rightarrow> 'a \<Rightarrow> 'b \<Rightarrow> 'a \<Rightarrow> 'b list" where
   \<open>append_update W L a = W(L:= W (L) @ [a])\<close>
 
 lemma append_ll_append_update:
@@ -1868,8 +1860,8 @@ definition find_unassigned_lit_wl_D :: \<open>_\<close> where
 sepref_register N\<^sub>0'
 declare N_hnr'[sepref_fr_rules]
 
-lemma N_hnr[sepref_import_param]: "(N\<^sub>0_code,N\<^sub>0')\<in>\<langle>unat_lit_rel\<rangle>list_rel"
-  using lits_less_upperN unfolding N\<^sub>0'_def N\<^sub>0_code_def
+lemma N_hnr[sepref_import_param]: "(N\<^sub>0,N\<^sub>0')\<in>\<langle>unat_lit_rel\<rangle>list_rel"
+  using lits_less_upperN unfolding N\<^sub>0'_def
   by (auto simp del: literal_of_nat.simps simp: p2rel_def lit_of_natP_def
       unat_lit_rel_def uint32_nat_rel_def nat_lit_rel_def br_def Collect_eq_comp
       list_rel_def list_all2_op_eq_map_right_iff  
